qlock-tactic3.lean
@@ -1,0 +1,113 @@
+/-
+Objective: Decoupling unification steps from rest of the proof
+-/
+
+import Bakery.DMC3
+import Bakery.command
+
+import Mathlib.Data.Multiset.Basic
+import Mathlib.Data.Multiset.AddSub
+
+
+
+/- EXAMPLE 1 -/
+namespace ex1
+
+structure Conf where
+  n : Multiset Nat
+  w : Multiset Nat
+  c : Multiset Nat
+  q : List Nat
+instance : State Conf := ⟨⟩
+
+
+inductive step_n2w : Transition Conf where
+  | mk : ∀ (i : Nat) (n w c : Multiset Nat) (q : List Nat),
+      step_n2w ⟨ i ::ₘ n, w, c, q ⟩ ⟨ n, i ::ₘ w, c, q ++ [i] ⟩
+
+inductive step_c2n : Transition Conf where
+  | mk : ∀ (i : Nat) (n w c : Multiset Nat) (q : List Nat),
+      step_c2n ⟨ n, w, i ::ₘ c, i :: q ⟩ ⟨ i ::ₘ n, w, c, q ⟩
+
+def pat1 : Pattern Conf := fun cf =>
+  ∃ (U W : Multiset Nat) (Q : List Nat),
+    cf = ⟨ U, W, ∅, Q ⟩
+    ∧ U + W ≠ ∅
+    ∧ Multiset.Nodup (U + W)
+    ∧ ↑Q = W
+
+
+-- Generic Adapter: uses outParam to represent the unifier (positive case) / ⊥ (negative case)
+class Unify (c1 c2 : Conf) (Result : outParam Prop) where
+  resolve : c1 = c2 → Result
+
+
+
+
+/-
+  NEGATIVE CASE: non-unifiable
+-/
+
+-- unification proof
+instance {N N' W' C' : Multiset ℕ} {Q Q' : List ℕ} {i : Nat} :
+  Unify
+    { n := N', w := W', c := i ::ₘ C', q := i :: Q' }
+    { n := N, w := ↑Q, c := 0, q := Q }
+    False where
+  resolve h_unify := by
+    injection h_unify; simp_all
+
+-- ∀ st st', pat1 st → step_c2n st st' → ⊥ st'
+lemma _1c0 : (↑step_c2n : Transformer Conf) pat1 ⊥ := by
+  -- boilerplate: unpacking the pattern and the step
+  intro s s' h_s step
+  simp [pat1] at h_s
+  obtain ⟨N, Q, h_unify, h_s1, h_s2⟩ := h_s
+  rcases step
+
+  -- { n := n✝, w := w✝, c := i✝ ::ₘ c✝, q := i✝ :: q✝ } = { n := N, w := ↑Q, c := 0, q := Q }
+  obtain unifier := Unify.resolve h_unify
+
+  /- the unifier returned false, so complete the proof -/
+  assumption
+
+
+
+
+
+
+/-
+  POSITIVE CASE: unifiable
+-/
+
+-- unification proof
+instance {N N' W' C' : Multiset ℕ} {Q Q' : List ℕ} {i : Nat} :
+  Unify
+    { n := i ::ₘ N', w := W', c := C', q := Q' }
+    { n := N, w := ↑Q, c := 0, q := Q }
+    ((i ::ₘ N' = N) ∧ (W' = ↑Q) ∧ (C' = 0) ∧ (Q' = Q)) where
+  resolve h_unify := by
+    injection h_unify with hn hw hc hq
+    exact ⟨hn, hw, hc, hq⟩
+
+
+-- ∀ st st', pat1 st → step_n2w st st' → pat1 st'
+lemma _1a1 : (↑step_n2w : Transformer Conf) pat1 pat1 := by
+  -- boilerplate: unpacking the pattern and the step
+  intro s s' ps step
+  simp [pat1] at ps
+  obtain ⟨N, Q, h_unify, h_s1, h_s2⟩ := ps
+  rcases step
+
+  -- { n := i✝ ::ₘ n✝, w := w✝, c := c✝, q := q✝ } = { n := N, w := ↑Q, c := 0, q := Q }
+  obtain unifier := Unify.resolve h_unify
+
+  /- unifier exists, so continue the proof with bindings added to hypothesis -/
+  simp [pat1]
+  refine ⟨?_, ?_, ?_⟩
+
+  · sorry
+  · sorry
+  · sorry
+
+end ex1
